% !TEX root = ../main.tex

Before starting to analyse the terms, we need to set up
\subsection{Absence of sources}
\label{sub:Absence of sources}
The described cumulant method shall not have any sources and sinks and be incompressible. Hence
\begin{equation}
    \rho  = m_{00} = m_{00}^*
\end{equation}
and thus
\begin{equation}
    \rho = m_{00}^{(p)} = m_{00}^{*^{(p)}}
\end{equation}

Velocity is no conserved quantity in our setting, because forcing terms like gravity can alter it.

\subsection{Zeroth order moments are constant in space}
\label{sub:Zeroth order moments are constant in space}
Zeroth order terms are independent of our expansion parameter $\epsilon$ and thus have to be constant in space. Hence
\begin{equation}
  \partial_x m_{\alpha\beta}^{(0)} = 0
\end{equation}
\begin{equation}
  \partial_y m_{\alpha\beta}^{(0)} = 0
\end{equation}


\subsection{Collision invariants}
\label{sub:Collision invariants}
As the zeroth order terms of the expansion have to be constant in space, we get
\begin{equation}
  \label{eq:first order collision invariant}
  \begin{aligned}
    m_{\alpha\beta}^{(1)}
    & = m_{\alpha\beta}^{*^{(1)}}
    - \partial_x m_{(\alpha+1)\beta}^{*^{(0)}}
    - \partial_y m_{\alpha(\beta+1)}^{*^{(0)}} \\
    & = m_{\alpha\beta}^{*^{(1)}}
  \end{aligned}
\end{equation}
Thus, all moments of order zero,~\eqref{eq:zeroth order in epsilon},
and one,~\eqref{eq:first order collision invariant}, in $\epsilon$, are collision invariants.

\subsection{Collision of moments}
\label{sub:Collision of moments}
Last but not least, we take a look at the collision and insert the findings of Section~\ref{sub:Expanding the normalized cumulants}.
Starting from~\eqref{eq:collision equation system full}, multiplying by $m_{00}$ we get
\begin{equation}
  \begin{aligned}
    K_{11}^{*} & = (1-\omega_1)K_{11} \\
    K_{20}^{*} - K_{02}^{*} & = (1-\omega_1) (K_{20} - K_{02}) \\
    K_{20}^{*} + K_{02}^{*} & = (1-\omega_2) (K_{20} + K_{02}) + \omega_2 \frac{2 m_{00}^{(1)}}{3} \\
    K_{21}^{*} & = (1-\omega_3)K_{21} \\
    K_{12}^{*} & = (1-\omega_3)K_{12} \\
    K_{22}^{*} & = (1-\omega_4)K_{22}.
  \end{aligned}
\end{equation}
now, insert the moment representations at first order to get
\begin{equation}
  \begin{aligned}
    m_{11}^{(1)*}
    & = (1-\omega_1)m_{11}^{(1)} \\
%
    m_{20}^{(1)*} - m_{02}^{(1)*}
    & = (1-\omega_1) (m_{20}^{(1)} - m_{02}^{(1)}) \\
%
    m_{20}^{(1)*} + m_{02}^{(1)*}
    & = (1-\omega_2) (m_{20}^{(1)} + m_{02}^{(1)}) + \omega_2 \frac{2 m_{00}^{(1)}}{3} \\
%
    m_{21}^{(1)*} - \theta m_{01}^{(1)*}
    & = (1-\omega_3)(m_{21}^{(1)} - \theta m_{01}^{(1)}) \\
%
    m_{12}^{(1)*} - \theta m_{10}^{(1)*}
    & = (1-\omega_3)(m_{12}^{(1)} - \theta m_{01}^{(1)}) \\
%
m_{22}^{(1)}
  - \theta (m_{20}^{(1)} + m_{02}^{(1)})
  - 2\frac{ m_{10}^{(1)} m_{12}^{(0)} }{m_{00}^{(0)}}&\\
  - 2\frac{ m_{21}^{(0)} m_{01}^{(1)} }{m_{00}^{(0)}}
  - 4\frac{ m_{11}^{(1)} m_{11}^{(0)} }{m_{00}^{(0)}}
    & = (1-\omega_4)\bigg(m_{22}^{(1)}
      - \theta (m_{20}^{(1)} + m_{02}^{(1)})
      \\&\quad
      - 2\frac{ m_{10}^{(1)} m_{12}^{(0)} }{m_{00}^{(0)}}
      - 2\frac{ m_{21}^{(0)} m_{01}^{(1)} }{m_{00}^{(0)}}
      \\&\quad
      - 4\frac{ m_{11}^{(1)} m_{11}^{(0)} }{m_{00}^{(0)}}\bigg) \\
  \end{aligned}
\end{equation}
Inserting the second order approximations
\begin{equation}
  \begin{aligned}
    m_{11}^{(2)*} - \frac{ m_{10}^{(1)*}m_{01}^{(1)*}}{m_{00}^{(0)*}} & = (1-\omega_1)\left(m_{11}^{(2)} - \frac{ m_{10}^{(1)}m_{01}^{(1)}}{m_{00}^{(0)}}\right) \\
    m_{20}^{(2)*}-m_{02}^{(2)*} - \frac{ m_{10}^{(1)*2} - m_{01}^{(1)*2}}{m_{00}^{(0)*}} & = (1-\omega_1) \left(m_{20}^{(2)}-m_{02}^{(2)} - \frac{ m_{10}^{(1)2} - m_{01}^{{(1)}^2}}{m_{00}^{(0)}}\right) \\
    %
    m_{20}^{(2)*}+m_{02}^{(2)*} - \frac{ m_{10}^{(1)*2} + m_{01}^{(1)*2}}{m_{00}^{(0)*}} & = (1-\omega_2)
    \left(m_{20}^{(2)}+m_{02}^{(2)} - \frac{ m_{10}^{(1)2} + m_{01}^{{(1)}^2}}{m_{00}^{(0)}}\right)
    \\&\quad
    + \omega_2 \frac{2 m_{00}^{(2)}}{3} \\
  \end{aligned}
\end{equation}

\paragraph{Reduced case}
\label{par:Reduced case}
In the reduced case where only $\omega_1$ is not one, we get
\begin{equation}
  \begin{aligned}
    m_{11}^{(1)*} & = (1-\omega_1) m_{11}^{(1)} \\
    m_{20}^{(1)*} - m_{02}^{(1)*}
      & = (1-\omega_1) (m_{20}^{(1)} - m_{02}^{(1)}) \\
    m_{20}^{(1)*} + m_{02}^{(1)*}
      & =  \frac{2 m_{00}^{(1)}}{3} \\
    m_{21}^{(1)*} & = \theta m_{01}^{(1)*} = \theta m_{01}^{(1)} \\
    m_{12}^{(1)*} & = \theta m_{10}^{(1)*} = \theta m_{10}^{(1)} \\
    m_{22}^{(1)*} & =  \theta (m_{20}^{(1)} + m_{02}^{(1)})
      + 2\frac{ m_{10}^{(1)} m_{12}^{(0)} }{m_{00}^{(0)}}
      \\&\quad
      + 2\frac{ m_{21}^{(0)} m_{01}^{(1)} }{m_{00}^{(0)}}
      + 4\frac{ m_{11}^{(1)} m_{11}^{(0)} }{m_{00}^{(0)}}
      \\&= \theta \frac{2 m_{00}^{(1)}}{3} + 2\frac{ m_{10}^{(1)} m_{12}^{(0)} }{m_{00}^{(0)}}
      \\&\quad
      + 2\frac{ m_{21}^{(0)} m_{01}^{(1)} }{m_{00}^{(0)}}
      + 4\frac{ m_{11}^{(1)} m_{11}^{(0)} }{m_{00}^{(0)}}
  \end{aligned}
\end{equation}
And finally, inserting the second order terms into the first three equations
\begin{equation}
  \begin{aligned}
    m_{11}^{(2)*} - \frac{ m_{10}^{(1)*}m_{01}^{(1)*}}{m_{00}^{(0)*}} & = (1-\omega_1)\left(m_{11}^{(2)} - \frac{ m_{10}^{(1)}m_{01}^{(1)}}{m_{00}^{(0)}}\right) \\
    m_{20}^{(2)*}-m_{02}^{(2)*} - \frac{ m_{10}^{(1)*2} - m_{01}^{(1)*2}}{m_{00}^{(0)*}} & = (1-\omega_1) \left(m_{20}^{(2)}-m_{02}^{(2)} - \frac{ m_{10}^{(1)2} - m_{01}^{{(1)}^2}}{m_{00}^{(0)}}\right) \\
    %
    m_{20}^{(2)*}+m_{02}^{(2)*} - \frac{ m_{10}^{(1)*2} + m_{01}^{(1)*2}}{m_{00}^{(0)*}} & = \frac{2 m_{00}^{(2)}}{3}
  \end{aligned}
\end{equation}

\subsection{Equilibrium in terms of moments}
\label{sub:Equilibrium in terms of moments}
We can also define our equilibrium cumulants in terms of moments.
First of all, we start with combining~\eqref{eq:definition of kappa_00} with the first equation in~\eqref{eq:equilibrium cumulants}, which results in
\begin{equation}
  \begin{aligned}
    {\ln(m_{00})}^{eq} &= {\ln(m_{00})}^{eq} \\
    \Leftrightarrow\quad m_{00}^{eq} &= m_{00}^{eq} \\
    \Leftrightarrow\quad m_{00}^{eq(p)} &= m_{00}^{eq(p)} \quad\forall p\ge 0
  \end{aligned}
\end{equation}
Starting from~\eqref{eq:equilibrium cumulants}, multiplying by $m_{00}$ and inserting our known values, we get
\begin{equation}
  \begin{aligned}
    m_{10}^{eq} & = m_{10} \\
    m_{01}^{eq} & = m_{01} \\
    m_{11}^{eq} - \frac{m_{10}^{eq}m_{01}^{eq}}{m_{00}} & = 0 \\
    m_{20}^{eq} - \frac{m_{10}^{{eq}^2}}{m_{00}} & = \frac{1}{3} m_{00} \\
    m_{02}^{eq} - \frac{m_{01}^{{eq}^2}}{m_{00}} & = \frac{1}{3} m_{00} \\
    m_{21}^{eq} - \frac{m_{20}^{eq}m_{01}^{eq}}{m_{00}} - 2\frac{m_{10}^{eq}m_{11}^{eq}} {m_{00}} + 2\frac{m_{10}^{{eq}^2} m_{01}^{eq}}{m_{00}^2} & = 0 \\
    m_{12}^{eq} - \frac{m_{10}^{eq}m_{02}^{eq}}{m_{00}}
    - 2\frac{m_{11}^{eq}m_{01}^{eq}}{m_{00}} + 2\frac{m_{10}^{eq} m_{01}^{{eq}^2}}{m_{00}^2} & = 0 \\
    m_{22}^{eq} &\\
    - 2 \frac{m_{10}^{eq}m_{12}^{eq}}{m_{00}} - 2\frac{m_{21}^{eq}m_{01}^{eq}}{m_{00}}
    - 2 \frac{m_{11}^{{eq}^2}}{m_{00}} - \frac{m_{20}^{eq}m_{02}^{eq}}{m_{00}} &\\
    + 2 \frac{m_{10}^{{eq}^2} m_{02}^{eq}}{m_{00}^2} + 8 \frac{m_{10}^{eq}m_{11}^{eq}m_{01}} {m_{00}^2}
    + 2 \frac{m_{20}^{eq}m_{01}^{{eq}^2}}{m_{00}^2} &\\
    - 6 \frac{m_{10}^{{eq}^2} m_{01}^{{eq}^2}}{m_{00}^{{eq}^3}} & = 0.
  \end{aligned}
\end{equation}
Zeroth order:
\begin{equation}
  \begin{aligned}
    m_{10}^{eq^{(0)}} & = m_{10}^{(0)} = 0 \\
    m_{01}^{eq^{(0)}} & = 0 \\
    m_{11}^{eq^{(0)}} & = 0 \\
    m_{20}^{eq^{(0)}} & = \frac{1}{3} m_{00}^{(0)} \\
    m_{02}^{eq^{(0)}} & = \frac{1}{3} m_{00}^{(0)} \\
    m_{21}^{eq^{(0)}} & = 0 \\
    m_{12}^{eq^{(0)}} & = 0 \\
    m_{22}^{eq^{(0)}} - \theta m_{00}^{(0)} - 2\frac{ m_{11}^{eq(0)2}}{m_{00}^{(0)}} & = 0 \\
    \Leftrightarrow\quad m_{22}^{eq^{(0)}} &= \frac{1}{3} m_{00}^{(0)}.
  \end{aligned}
\end{equation}
In the first order case, it looks like
\begin{equation}
  \begin{aligned}
    m_{10}^{eq^{(1)}} & = m_{10}^{(1)} \\
    m_{01}^{eq^{(1)}} & = m_{01}^{(1)} \\
    m_{11}^{eq^{(1)}} & = 0 \\
    m_{20}^{eq^{(1)}} & = \frac{1}{3} m_{00}^{(1)} \\
    m_{02}^{eq^{(1)}} & = \frac{1}{3} m_{00}^{(1)} \\
    m_{21}^{eq^{(1)}} & = \theta m_{01}^{eq^{(1)}} = \theta m_{01}^{(1)}\\
    m_{12}^{eq^{(1)}} & = \theta m_{10}^{eq^{(1)}} = \theta m_{10}^{(1)} \\
    m_{22}^{eq^{(1)}} - \theta (m_{20}^{eq^{(1)}} + m_{02}^{eq^{(1)}})
    - 2\frac{ m_{10}^{eq^{(1)}} m_{12}^{eq^{(0)}} }{m_{00}^{(0)}}&\\
    - 2\frac{ m_{21}^{eq^{(0)}} m_{01}^{eq^{(1)}} }{m_{00}^{(0)}}
    - 4\frac{ m_{11}^{eq^{(1)}} m_{11}^{eq^{(0)}} }{m_{00}^{(0)}}&=0\\
    m_{22}^{eq^{(1)}} &= \frac{2}{9} m_{00}^{(1)}
    + \frac{2}{3}\frac{  m_{10}^{(1)2} +m_{01}^{(1)2} }{m_{00}^{(0)}}
  \end{aligned}
\end{equation}
\todo[inline]{remark: in 3D this would be much nicer, as we would get 3 components and finally $\frac{1}{3} m_{00}^{(1)} + \ldots$}
and the second order
\begin{equation}
  \begin{aligned}
    m_{11}^{eq^{(2)}} & = \frac{ m_{10}^{eq^{(1)}}m_{01}^{eq^{(1)}}}{m_{00}^{(0)}} \\
    m_{20}^{eq^{(2)}} - \frac{ m_{10}^{eq(1)2}}{m_{00}^{(0)}} & = \frac{1}{3} m_{00}^{(2)} \\
    m_{02}^{eq^{(2)}} - \frac{ m_{01}^{eq(1)2}}{m_{00}^{(0)}} & = \frac{1}{3} m_{00}^{(2)}
  \end{aligned}
\end{equation}
