\documentclass{article}
\usepackage[utf8]{inputenc}
\usepackage{mathtools}

%\input{../../latex_basics/definitions}

\begin{document}
We know:
\begin{equation}
  K_{11} = m_{11} - \frac{m_{10}m_{01}}{m_{00}}
\end{equation}
We can expand $K$ for expansion parameter $\epsilon$ to get our known series expansion
\begin{equation}
  K_{11} = \sum_{i=0}^\infty \epsilon^i K_{11}^{(i)}
\end{equation}
If I now want to compute, let's say, $K_{11}^{(2)}$ in terms of expanded moments, I'd say we have to do

\begin{equation}
  \begin{aligned}
    K_{11} & = m_{11} - \frac{m_{10}m_{01}}{m_{00}}\\
    \Leftrightarrow
    \sum_{i=0}^\infty \epsilon^i K_{11}^{(i)}
    & = \sum_{i=0}^\infty \epsilon^i m_{11}^{(i)} -
    \frac{\sum_{i,j=0}^\infty \epsilon^{i+j} m_{10}^{(i)}m_{01}^{(j)}}
         {\sum_{i=0}^\infty \epsilon^i m_{00}^{(i)}}
  \end{aligned}
\end{equation}
and match the $\epsilon$ coefficient on both sides. This obviously will be not possible, thanks to the sum in the denominator.
In the paper, he states
\begin{equation}
  K_{11}^{(2)}
  = m_{11}^{(2)} -
  \frac{m_{10}^{(1)}m_{01}^{(1)}}
       {m_{00}^{(0)}}
\end{equation}
Which obviously has same $\epsilon$ coefficients on both sides, but I can't see, why this is the right way to do it?
If we just ignore the sum in the denominator, I would suggest the expansion to be
\begin{equation}
  K_{11}^{(2)}
  = m_{11}^{(2)} -
  \frac{m_{10}^{(1)}m_{01}^{(1)}+m_{10}^{(0)}m_{01}^{(2)}+m_{10}^{(2)}m_{01}^{(0)}}
       {m_{00}^{(0)}}
\end{equation}
Why should I not be allowed to match $*^{(0)}$ and $*^{(2)}$. Sure, they are on different scales, but I suppose they can be combined, anyway.
In the Geier Paper, it's (G.29) ff.

\section{geometric series}
\label{sec:geometric series}
\begin{equation}
  \begin{aligned}
    K_{11} & = m_{11} - \frac{m_{10}m_{01}}{m_{00}}\\
    \Leftrightarrow
    \sum_{i=0}^\infty \epsilon^i K_{11}^{(i)}
    & = \sum_{i=0}^\infty \epsilon^i m_{11}^{(i)} -
    \frac{\sum_{i,j=0}^\infty \epsilon^{i+j} m_{10}^{(i)}m_{01}^{(j)}}
        {\sum_{i=0}^\infty \epsilon^i m_{00}^{(i)}}\\
    \Leftrightarrow
    \sum_{i=0}^\infty \epsilon^i K_{11}^{(i)}
    & = \sum_{i=0}^\infty \epsilon^i m_{11}^{(i)} -
    \frac{\sum_{i,j=0}^\infty \epsilon^{i+j} m_{10}^{(i)}m_{01}^{(j)}}
        {m_{00}^{(0)}}
        \frac{1}{1 - \sum_{i=1}^\infty \epsilon^i \frac{ - m_{00}^{(i)}}{ m_{00}^{(0)}}}\\
    \Leftrightarrow
    \sum_{i=0}^\infty \epsilon^i K_{11}^{(i)}
    & = \sum_{i=0}^\infty \epsilon^i m_{11}^{(i)} -
    \frac{\sum_{i,j=0}^\infty \epsilon^{i+j} m_{10}^{(i)}m_{01}^{(j)}}
        {m_{00}^{(0)}}
    \sum_{j=0}^\infty {\left(\sum_{i=1}^\infty \epsilon^i \frac{ - m_{00}^{(i)}}{ m_{00}^{(0)}}\right)}^j
  \end{aligned}
\end{equation}
Second order terms
\begin{equation}
  \begin{aligned}
    K_{11}^{(2)}
    &= m_{11}^{(2)} \\
    &\quad-
    \frac{
      m_{10}^{(1)}m_{01}^{(1)}
    + m_{10}^{(0)}m_{01}^{(2)}
    + m_{10}^{(2)}m_{01}^{(0)}
    }{m_{00}^{(0)}}\\
    &\quad
    -(m_{10}^{(1)}m_{01}^{(0)} + m_{10}^{(0)}m_{01}^{(1)}) m_{00}^{(1)}\\
    &\quad
    - m_{10}^{(0)}m_{01}^{(0)}
    \left(
      \underbrace{m_{00}^{(2)}}_{j=1,i=2}
      - \underbrace{\frac{m_{00}^{(2)2}}{m_{00}^{(0)}}}_{j=2,i=1}
    \right)\\
    &= m_{11}^{(2)} \\
    &\quad-
    \frac{
      m_{10}^{(1)}m_{01}^{(1)}
    + m_{10}^{(0)}m_{01}^{(2)}
    + m_{10}^{(2)}m_{01}^{(0)}
    + m_{10}^{(0)}m_{01}^{(0)}m_{00}^{(2)2}
    }{m_{00}^{(0)}}\\
    &\quad
    - m_{00}^{(1)}(m_{10}^{(1)}m_{01}^{(0)} + m_{10}^{(0)}m_{01}^{(1)}) \\
    &\quad
    - m_{00}^{(2)}m_{10}^{(0)}m_{01}^{(0)}
  \end{aligned}
\end{equation}

\end{document}
