\documentclass{article}
\usepackage[utf8]{inputenc}
\input{../../latex_basics/definitions}


\title{Notes concerning the paper}
\author{Florian Rohm}


\begin{document}
\maketitle

\begin{abstract}
\end{abstract}

\section{Definitions}
\label{sec:Definitions}

Laplace operator:
\begin{equation}
  \label{eq:Definition of Laplace}
  \mathcal{L}[g](\Xi) = \int_{-\infty}^\infty g(\xi) e^{-\Xi \cdot \xi}d\xi
\end{equation}

Continuous definition of f using the Diraque delta
\begin{equation}
  \label{eq:Definition of f xi}
  f(\xi) = \sum_{i,j} f_{ij}\delta(ic - \xi_1)\delta(jc - \xi_2)
\end{equation}
Definition of the Laplace transform of $f$
\begin{equation}
  \label{eq:Definition of F}
  \begin{aligned}
    F(\Xi_1, \Xi_2) & = \mathcal{L}[f](\Xi) = \int_{-\infty}^\infty f(\xi) e^{-\Xi \cdot \xi}d\xi \\
     & = \sum_{i,j}f_{ij} e^{-\Xi_1 ic} e^{-\Xi_2 jc}
  \end{aligned}
\end{equation}
Definition of the moments of $f$
\begin{equation}
  \label{eq:Definition of moments}
  m_{\alpha\beta} = \sum_{ij} i^\alpha j^\beta f_{ij}
\end{equation}
Taylor expansion of $F$
\begin{equation}
  \label{eq: taylor of F}
  \begin{aligned}
    F(\Xi_1, \Xi_2) & = \sum_{\alpha,\beta} \frac{1}{\alpha!\beta!} \frac{\partial^\alpha\partial^\beta}{{(\partial \Xi_1)}^\alpha{(\partial \Xi_2)}^\beta} F(\Xi_1, \Xi_2)\Bigr|_{\Xi_1=\Xi_2 = 0} \Xi_1^\alpha \Xi_2^\beta \\
    & = \sum_{\alpha,\beta} \frac{1}{\alpha!\beta!} \frac{\partial^\alpha\partial^\beta}
      {{(\partial \Xi_1)}^\alpha{(\partial \Xi_2)}^\beta}  \sum_{i,j}f_{ij} e^{-\Xi_1 ic} e^{-\Xi_2 jc} \Bigr|_{\Xi_1=\Xi_2 = 0} \Xi_1^\alpha \Xi_2^\beta \\
    & = \sum_{\alpha,\beta} \frac{1}{\alpha!\beta!} {(-c)}^{\alpha+\beta}  \sum_{i,j} i^\alpha j^\beta f_{ij} e^{-\Xi_1 ic} e^{-\Xi_2 jc} \Bigr|_{\Xi_1=\Xi_2 = 0} \Xi_1^\alpha \Xi_2^\beta \\
    & = \sum_{\alpha,\beta} \frac{1}{\alpha!\beta!} {(-c)}^{\alpha+\beta}  \sum_{i,j} i^\alpha j^\beta f_{ij} \Xi_1^\alpha \Xi_2^\beta \\
    & = \sum_{\alpha,\beta} \frac{1}{\alpha!\beta!} {(-c)}^{\alpha+\beta}  m_{\alpha\beta} \Xi_1^\alpha \Xi_2^\beta
  \end{aligned}
\end{equation}

Hence,
\begin{equation}
  \label{eq:alternative representation of moments}
  m_{\alpha\beta} = {(-c)}^{-\alpha-\beta} \frac{\partial^\alpha\partial^\beta}{{(\partial \Xi_1)}^\alpha{(\partial \Xi_2)}^\beta} F(\Xi_1, \Xi_2)\Bigr|_{\Xi_1=\Xi_2 = 0}
\end{equation}
and $F(\Xi_1, \Xi_2)$ is the moment generating function of $f(\xi_1, \xi_2)$.

Cumulants are defined as the coefficients of the Taylor-expansion of the logarithm of the moment generating function:
\begin{equation}
  \label{eq:Definition of cumulants}
  c_{\alpha\beta} = {(-c)}^{-\alpha-\beta} \frac{\partial^\alpha\partial^\beta}{{(\partial \Xi_1)}^\alpha{(\partial \Xi_2)}^\beta} \ln(F(\Xi_1, \Xi_2))\Bigr|_{\Xi_1=\Xi_2 = 0}
\end{equation}

\section{Lattice Boltzmann Equation for D2Q9}
\label{sec:Lattice Boltzmann Equation for D2Q9}

Velocities are given by
\begin{equation}
  c_{ij}= \begin{pmatrix}i \\ j\end{pmatrix}, \quad i,j\in \{-1, 0, 1\}
\end{equation}
With $c$ defined as the cell width, the lattice Boltzmann equation is given by
\begin{equation}
  f_{ij}(t + \Delta t, x + i\Delta x , y + j\Delta y) = f^*_{ij}(t,x,y), \quad i,j\in \{-1, 0, 1\}
\end{equation}
or equivalently by shifting $x$ and $y$
\begin{equation}
  \label{eq:Lattice Boltzmann Equation}
  f_{ij}(t + \Delta t, x, y) = f^*_{ij}(t,x - i\Delta x , y - j\Delta y), \quad i,j\in \{-1, 0, 1\}
\end{equation}
where $f_{ij}$ are the pre-collission distributions and $f^*_{ij}$ the post collission distributions.

\section{Asymptotic Analysis}
\label{sec:Asymptotic Analysis}
\subsection{Preparation}
\label{sub:Preparation}

A Taylor expansion of~\eqref{eq:Lattice Boltzmann Equation} in both time and space gives
\begin{equation*}
  \sum_{\tau = 0}^\infty \frac{{\Delta t}^\tau }{\tau!} \frac{\partial^\tau}{{\partial t}^\tau} f_{ij}(t, x, y) =
  \sum_{m,n = 0}^\infty \frac{{(-i\Delta x)}^m{(-j\Delta x)}^n} {m!n!} \frac{\partial^m \partial^n}{ {\partial x}^m{\partial y}^n} f^*_{ij}(t, x, y)
\end{equation*}
which is equivalent to
\begin{equation}
  \label{eq:Taylor LB1}
  \sum_{\tau = 0}^\infty \frac{{\Delta t}^\tau }{\tau!} \frac{\partial^\tau}{{\partial t}^\tau} f_{ij}(t, x, y) =
    \sum_{m,n = 0}^\infty \frac{{(-c\Delta t)}^{m+n}} {m!n!} \frac{\partial^m \partial^n}{ {\partial x}^m{\partial y}^n} i^m j^n f^*_{ij}(t, x, y),
\end{equation}
using $\frac{\Delta x} {\Delta{t}} = c$.

Equation~\eqref{eq:Taylor LB1} holds for all $f_{ij}$ and thus also for all linear combinations
\begin{equation*}
  \sum_{k}\lambda_k f_{ij},
\end{equation*}
especially for those, which yield the moments, $m_{\alpha\beta} $, of $f$:
\begin{equation*}
  \sum_{k}\lambda_k f_{ij} = \sum_{i,j}i^\alpha j^\beta f_{ij}.
\end{equation*}
Therefore, we rewrite the system of equations for the $f_{ij}$ to a system of equations for the $m_{\alpha\beta}$.

\begin{align}
    \nonumber
    & & \sum_{ij} \sum_{\tau = 0}^\infty \frac{{\Delta t}^\tau }{\tau!} \frac{\partial^\tau}{{\partial t}^\tau} i^\alpha j^\beta f_{ij} &=
    \sum_{ij}\sum_{m,n = 0}^\infty \frac{i^m j^n {(-c\Delta t)}^{m+n}} {m!n!} \frac{\partial^m \partial^n}{ {\partial x}^m{\partial y}^n}i^\alpha j^\beta f^*_{ij}\\
    \nonumber
    &\Leftrightarrow &
    \sum_{\tau = 0}^\infty \frac{{\Delta t}^\tau }{\tau!} \frac{\partial^\tau}{{\partial t}^\tau} \sum_{ij}i^\alpha j^\beta f_{ij} &=
    \sum_{m,n = 0}^\infty \frac{{(-c\Delta t)}^{m+n}} {m!n!} \frac{\partial^m \partial^n}{ {\partial x}^m{\partial y}^n}\sum_{ij}i^{(\alpha + m)} j^{(\beta+n)} f^*_{ij}\\
      \label{eq: Taylor of moments}
     &\Leftrightarrow &
     \sum_{\tau = 0}^\infty \frac{{\Delta t}^\tau }{\tau!} \frac{\partial^\tau}{{\partial t}^\tau} m_{\alpha\beta} &=
    \sum_{m,n = 0}^\infty \frac{{(-c\Delta t)}^{m+n}} {m!n!} \frac{\partial^m \partial^n}{ {\partial x}^m{\partial y}^n} m^*_{(\alpha + m)(\beta + n)}
\end{align}
For the scale analysis, we introduce a dimensionless scaling parameter $\epsilon$.
Adapting the widely used diffusive scaling, we nondimensionalize the equations with characteristic length and timescales, $L$ and $\iota$
\begin{equation}
  \label{eq:nondimensionalisation}
  \begin{aligned}
    \Delta x & = L\epsilon \\
    \Delta t & = \iota\epsilon^2 \\
    c & = \frac{L}{\iota\epsilon} \\
    \{x, y\} & \rightarrow \{\frac{x}{L}, \frac{y}{L}\} \\
    t & \rightarrow \frac{t}{\iota}.
  \end{aligned}
\end{equation}
Additionally, the moments are expanded according to the scale $\epsilon$
\begin{align}
    \label{eq:expansion of m}
    m_{\alpha\beta} & = \sum_{p=1}^{\infty} \epsilon^p m_{\alpha\beta}^{(p)} \\
    \label{eq:expansion of m*}
    m^*_{\alpha\beta} & = \sum_{p=1}^{\infty} \epsilon^p m_{\alpha\beta}^{*(p)}.
\end{align}
Those are not allowed to depend on $\epsilon$ neither implicitly nor explicitly.
Inserting~\eqref{eq:nondimensionalisation},~\eqref{eq:expansion of m} and~\eqref{eq:expansion of m*} into~\eqref{eq: Taylor of moments} yields
\begin{align}
  \sum_{\tau = 0}^\infty \frac{{\Delta t}^\tau }{\tau!} \frac{\partial^\tau}{{\partial t}^\tau} \sum_{p=1}^{\infty} \epsilon^p m_{\alpha\beta}^{(p)}  &=
 \sum_{m,n = 0}^\infty \frac{{(-c\Delta t)}^{m+n}} {m!n!} \frac{\partial^m \partial^n}{ {\partial x}^m{\partial y}^n} \sum_{p=1}^{\infty} \epsilon^p m_{(\alpha + m)(\beta + n)}^{*(p)}
\end{align}


\end{document}
