% !TEX root = ../thesis.tex
The only apparent relaxation parameter in the asymptotic analysis in Section~\ref{sec: Momentum equation} and following will be $\omega_1$ which plays the role of viscosity like in the single relaxation time.
All other terms are save to be set to one regarding the first order analysis.

With the speed of sound for the D2Q9
\todo[inline]{cite}\todo[inline]{speed of sound nachfragen}
calculated as  $c_s^2=\frac{1}{3}$ we get
\begin{equation}
  \label{eq:collision equation system}
  \begin{aligned}
    \kappa_{00}^{*} & = \kappa_{00} \\
    \kappa_{10}^{*} & = \kappa_{10} \\
    \kappa_{01}^{*} & = \kappa_{01} \\
    \kappa_{11}^{*} & = (1-\omega_1)\kappa_{11} \\
    \kappa_{20}^{*} - \kappa_{02}^{*}
      & = (1-\omega_1) (\kappa_{20} - \kappa_{02}) \\
    \kappa_{20}^{*} + \kappa_{02}^{*}
      & =  \frac{2}{3} \\
    \kappa_{21}^{*} & = 0 \\
    \kappa_{12}^{*} & = 0 \\
    \kappa_{22}^{*} & = 0
  \end{aligned}
\end{equation}
or equivalently
\begin{equation}
  \begin{aligned}
    \kappa_{00}^{*} & = \kappa_{00} \\
    \kappa_{10}^{*} & = \kappa_{10} \\
    \kappa_{01}^{*} & = \kappa_{01} \\
    \kappa_{11}^{*} & = (1-\omega_1)\kappa_{11} \\
    \kappa_{20}^{*} & = \frac{1}{3} + \frac{1}{2}(1-\omega_1) (\kappa_{20} - \kappa_{02}) \\
    \kappa_{02}^{*} & = \frac{1}{3} - \frac{1}{2}(1-\omega_1) (\kappa_{20} - \kappa_{02}) \\
    \kappa_{21}^{*} & = 0 \\
    \kappa_{12}^{*} & = 0 \\
    \kappa_{22}^{*} & = 0.
  \end{aligned}
\end{equation}

As we want to compute with the normalized cumulants,~\eqref{eq: definition normalized cumulants}, we need to multiply each line with $m_{00}$.
Hence, the final collision reads
\begin{equation}
  \begin{aligned}
    K_{00}^{*} & = K_{00} \\
    K_{10}^{*} & = K_{10} \\
    K_{01}^{*} & = K_{01} \\
    K_{11}^{*} & = (1-\omega_1)K_{11} \\
    K_{20}^{*} & = \frac{m_{00}}{3} + \frac{1}{2}(1-\omega_1) (K_{20} - K_{02}) \\
    K_{02}^{*} & = \frac{m_{00}}{3} - \frac{1}{2}(1-\omega_1) (K_{20} - K_{02}) \\
    K_{21}^{*} & = 0 \\
    K_{12}^{*} & = 0 \\
    K_{22}^{*} & = 0
  \end{aligned}
\end{equation}
in the case with only one relaxation parameter and
\begin{equation}
  \begin{aligned}
    K_{00}^{*} & = K_{00} \\
    K_{10}^{*} & = K_{10} \\
    K_{01}^{*} & = K_{01} \\
    K_{11}^{*} & = (1-\omega_1)K_{11} \\
    K_{20}^{*} & =  \frac{1}{2}(1-\omega_2) (K_{20} + K_{02}) + \omega_2 \frac{\rho}{3} + \frac{1}{2}(1-\omega_1) (K_{20} - K_{02}) \\
    K_{02}^{*} & = \frac{1}{2}(1-\omega_2) (K_{20} + K_{02}) + \omega_2 \frac{\rho}{3} - \frac{1}{2}(1-\omega_1) (K_{20} - K_{02}) \\
    K_{21}^{*} & = (1-\omega_3)K_{21} \\
    K_{12}^{*} & = (1-\omega_3)K_{12} \\
    K_{22}^{*} & = (1-\omega_4)K_{22}
  \end{aligned}
\end{equation}
when we consider all of them.
