% !TEX root = ../thesis.tex

Now, we can finally write a collision for this method.
We will do again a linear interpolation between our values and their equilibrium like in equation~\eqref{eq: post collision discrete}, leaving us with
\begin{equation}
  \kappa_{\alpha\beta}^* \defined \kappa_{\alpha\beta} + \omega_i \left( \kappa_{\alpha\beta}^{eq} - \kappa_{\alpha\beta} \right).
\end{equation}
This time though, we have no need to restrict ourselves to just one parameter, but chose one for each cumulant.
Hence, using~\eqref{eq: equilibrium cumulants}, we get the post collision cumulants $\kappa_{\alpha\beta}^*$
\begin{equation}
  \label{eq: post equilibrium cumulants}
  \begin{aligned}
    \kappa_{00}^{*} & = \kappa_{00} + \omega_1 \left( \ln(\rho) - \kappa_{00} \right) \\
    \kappa_{10}^{*} & = \kappa_{10} + \omega_2 \left( u_1 - \kappa_{10} \right) \\
    \kappa_{01}^{*} & = \kappa_{01} + \omega_3 \left( u_2 - \kappa_{01} \right) \\
    \kappa_{11}^{*} & = \kappa_{11} + \omega_4 \left( - \kappa_{11} \right) \\
    \kappa_{20}^{*} - \kappa_{02}^{*}
      & = (\kappa_{20} - \kappa_{02}) + \omega_5 \left( - \kappa_{20} + \kappa_{02} \right) \\
    \kappa_{20}^{*} + \kappa_{02}^{*}
      & = (\kappa_{20} + \kappa_{02}) + \omega_6 \left( 2 c_s^2 - \kappa_{20} - \kappa_{02} \right) \\
    \kappa_{21}^{*} & = \kappa_{21} + \omega_7 \left( - \kappa_{21} \right) \\
    \kappa_{12}^{*} & = \kappa_{12} + \omega_8 \left( - \kappa_{12} \right) \\
    \kappa_{22}^{*} & = \kappa_{22} + \omega_9 \left( - \kappa_{22} \right)
  \end{aligned}
\end{equation}
which can be simplified to
\begin{equation}
  \label{eq: collision final before simplification}
  \begin{aligned}
    \kappa_{00}^{*} & = \kappa_{00} \\
    \kappa_{10}^{*} & = \kappa_{10} \\
    \kappa_{01}^{*} & = \kappa_{01} \\
    \kappa_{11}^{*} & = (1-\omega_4)\kappa_{11} \\
    \kappa_{20}^{*} - \kappa_{02}^{*}
      & = (1-\omega_5) (\kappa_{20} - \kappa_{02}) \\
    \kappa_{20}^{*} + \kappa_{02}^{*}
      & = (1-\omega_6)(\kappa_{20} + \kappa_{02}) + \omega_6 \left( 2 c_s^2 \right) \\
    \kappa_{21}^{*} & = (1-\omega_7)\kappa_{21} \\
    \kappa_{12}^{*} & = (1-\omega_8)\kappa_{12} \\
    \kappa_{22}^{*} & = (1-\omega_9)\kappa_{22},
  \end{aligned}
\end{equation}
using equations~\eqref{eq: definition of kappa_00} to~\eqref{eq: definition of kappa_01} or equivalently
\begin{equation}
  \label{eq: collision final before simplification normalized}
  \begin{aligned}
    K_{00}^{*} & = K_{00} \\
    K_{10}^{*} & = K_{10} \\
    K_{01}^{*} & = K_{01} \\
    K_{11}^{*} & = (1-\omega_4)K_{11} \\
    K_{20}^{*} - K_{02}^{*}
      & = (1-\omega_5) (K_{20} - K_{02}) \\
    K_{20}^{*} + K_{02}^{*}
      & = (1-\omega_6)(K_{20} + K_{02}) + \omega_6 \left( 2 m_{00} c_s^2 \right) \\
    K_{21}^{*} & = (1-\omega_7)K_{21} \\
    K_{12}^{*} & = (1-\omega_8)K_{12} \\
    K_{22}^{*} & = (1-\omega_9)K_{22}.
  \end{aligned}
\end{equation}
The recovered post equilibrium values $\kappa_{20}^{*}$ and $\kappa_{02}^{*}$ can now be calculated
\begin{equation}
  \begin{pmatrix}
    \kappa_{20}^{*} \\
    \kappa_{02}^{*}
  \end{pmatrix}
  = \frac{1}{2}
  \begin{pmatrix}
    1 & 1 \\ -1 & 1
  \end{pmatrix}
  \begin{pmatrix}
    a\\
    b
  \end{pmatrix}
\end{equation}
where
\begin{equation}
 \begin{aligned}
   a \defined \kappa_{20}^{*} - \kappa_{02}^{*}
     & = (1-\omega_5) (\kappa_{20} - \kappa_{02}) \\
   b \defined \kappa_{20}^{*} + \kappa_{02}^{*}
     & = (1-\omega_6)(\kappa_{20}^{*} + \kappa_{02}^{*}) + \omega_6 2 c_s^2,
 \end{aligned}
\end{equation}
and analogously for the normalized form.
