% !TEX root = ../thesis.tex
Last but not least, we take a look at the collision and insert the findings of Section~\ref{sub: Expanding the normalized cumulants}.
Starting from~\eqref{eq: final collision one relaxation}, we insert the moment representations at first order to get
\begin{equation}
  \begin{aligned}
    m_{11}^{*^{(1)}} & = (1-\omega_1) m_{11}^{(1)} \\
    m_{20}^{*^{(1)}} - m_{02}^{*^{(1)}}
      & = (1-\omega_1) (m_{20}^{(1)} - m_{02}^{(1)}) \\
    m_{20}^{*^{(1)}} + m_{02}^{*^{(1)}}
      & =  \frac{2 m_{00}^{(1)}}{3} \\
    m_{21}^{*^{(1)}} & = \theta m_{01}^{*^{(1)}} = \theta m_{01}^{(1)} \\
    m_{12}^{*^{(1)}} & = \theta m_{10}^{*^{(1)}} = \theta m_{10}^{(1)} \\
    m_{22}^{*^{(1)}} & =  \theta (m_{20}^{(1)} + m_{02}^{(1)})
      + 2\frac{ m_{10}^{(1)} m_{12}^{(0)} }{m_{00}^{(0)}}
      \\&\quad
      + 2\frac{ m_{21}^{(0)} m_{01}^{(1)} }{m_{00}^{(0)}}
      + 4\frac{ m_{11}^{(1)} m_{11}^{(0)} }{m_{00}^{(0)}}
      \\&= \theta \frac{2 m_{00}^{(1)}}{3} + 2\frac{ m_{10}^{(1)} m_{12}^{(0)} }{m_{00}^{(0)}}
      \\&\quad
      + 2\frac{ m_{21}^{(0)} m_{01}^{(1)} }{m_{00}^{(0)}}
      + 4\frac{ m_{11}^{(1)} m_{11}^{(0)} }{m_{00}^{(0)}}
  \end{aligned}
\end{equation}
Additionally, we will need, inserting the second order terms into the first three equations
\begin{align}
  m_{11}^{*^{(2)}} - \frac{ m_{10}^{*^{(1)}}m_{01}^{*^{(1)}}}{m_{00}^{(0)*}} & = (1-\omega_1)\left(m_{11}^{(2)} - \frac{ m_{10}^{(1)}m_{01}^{(1)}}{m_{00}^{(0)}}\right) \\
  m_{20}^{*^{(2)}}-m_{02}^{*^{(2)}} - \frac{ m_{10}^{*^{{(1)}^2}} - m_{01}^{*^{{(1)}^2}}}{m_{00}^{(0)*}} & = (1-\omega_1) \left(m_{20}^{(2)}-m_{02}^{(2)} - \frac{ m_{10}^{{(1)}^2} - m_{01}^{{(1)}^2}}{m_{00}^{(0)}}\right) \\
  %
  m_{20}^{*^{(2)}}+m_{02}^{*^{(2)}} - \frac{ m_{10}^{*^{{(1)}^2}} + m_{01}^{*^{{(1)}^2}}}{m_{00}^{(0)*}} & = \frac{2 m_{00}^{(2)}}{3}
\end{align}
