% !TEX root = ../thesis.tex
This section will lay the foundation of the analysis by expanding~\eqref{eq: lattice boltzmann equation} into a Taylor series, identifying and expanding the moments.

First of all,~\eqref{eq: lattice boltzmann equation} is reformulated to
\begin{equation}
  \label{eq: lattice boltzmann equation shifted}
  f_{ij}(x, y, t + \Delta t) = f^*_{ij}(x - i \Delta x , y - j\Delta y, t), \quad\forall i,j\in \{-1, 0, 1\}
\end{equation}
by shifting $x$ and $y$. Now, a Taylor expansion of~\eqref{eq: lattice boltzmann equation shifted} in both time and space gives
\begin{equation*}
  \sum_{\tau = 0}^\infty \frac{{\Delta t}^\tau }{\tau!} \frac{\partial^\tau}{{\partial t}^\tau} f_{ij}(t, x, y) =
  \sum_{m,n = 0}^\infty \frac{{(-i\Delta x)}^m{(-j\Delta y)}^n} {m!n!} \frac{\partial^m \partial^n}{ {\partial x}^m{\partial y}^n} f^*_{ij}(t, x, y)
\end{equation*}
which is equivalent to
\begin{equation}
  \label{eq: Taylor LB1}
  \sum_{\tau = 0}^\infty \frac{{\Delta t}^\tau }{\tau!} \frac{\partial^\tau}{{\partial t}^\tau} f_{ij}(t, x, y) =
    \sum_{m,n = 0}^\infty \frac{{(-\Delta t)}^{m+n}} {m!n!} \frac{\partial^m \partial^n}{ {\partial x}^m{\partial y}^n} {(ci)}^m {(cj)}^n f^*_{ij}(t, x, y),
\end{equation}
using~\eqref{eq: relation between stepsizes}.

Equation~\eqref{eq: Taylor LB1} holds for all $f_{ij}$ and thus also for all linear combinations
\begin{equation*}
  \sum_{k}\lambda_k f_{ij},
\end{equation*}
especially for those, which yield the moments, $m_{\alpha\beta} $, of $f$:
\begin{equation}
  \sum_{k}\lambda_k f_{ij} = \sum_{i,j}c^{\alpha + \beta}i^\alpha j^\beta f_{ij}=m_{\alpha\beta}.
\end{equation}
Therefore, we rewrite the system of equations for the $f_{ij}$ to a system of equations for the $m_{\alpha\beta}$ like

\begin{align}
    \nonumber
    & & \sum_{ij} \sum_{\tau = 0}^\infty \frac{{\Delta t}^\tau }{\tau!} \frac{\partial^\tau}{{\partial t}^\tau} {(ci)}^\alpha {(cj)}^\beta f_{ij}
    &=
    \sum_{ij}\sum_{m,n = 0}^\infty \frac{{(-\Delta t)}^{m+n}} {m!n!} \frac{\partial^m \partial^n}{ {\partial x}^m{\partial y}^n} {(ci)}^m {(cj)}^n {(ci)}^\alpha {(cj)}^\beta f^*_{ij}
    \\ \nonumber &\equivalent &
    \sum_{\tau = 0}^\infty \frac{{\Delta t}^\tau }{\tau!} \frac{\partial^\tau}{{\partial t}^\tau} \sum_{ij}i^\alpha j^\beta f_{ij}
    &=
    \sum_{m,n = 0}^\infty \frac{{(-\Delta t)}^{m+n}} {m!n!} \frac{\partial^m \partial^n}{ {\partial x}^m{\partial y}^n}\sum_{ij}{(ci)}^{(\alpha+m)} {(cj)}^{(\beta+n)} f^*_{ij}
    \\ \nonumber &\equivalent &
     \sum_{\tau = 0}^\infty \frac{{\Delta t}^\tau }{\tau!} \frac{\partial^\tau}{{\partial t}^\tau} m_{\alpha\beta} &=
    \sum_{m,n = 0}^\infty \frac{{(-\Delta t)}^{m+n}} {m!n!} \frac{\partial^m \partial^n}{ {\partial x}^m{\partial y}^n} m^*_{(\alpha + m)(\beta + n)}
     \\  \label{eq: Taylor of moments} &\equivalent &
     \sum_{\tau = 0}^\infty \frac{{\Delta t}^\tau }{\tau!} \frac{\partial^\tau}{{\partial t}^\tau} \frac{m_{\alpha\beta}}{c^{\alpha + \beta}} &=
    \sum_{m,n = 0}^\infty \frac{{(- c\Delta t)}^{m+n}} {m!n!} \frac{\partial^m \partial^n}{ {\partial x}^m{\partial y}^n} \frac{m^*_{(\alpha + m)(\beta + n)}}{c^{\alpha + m + \beta + n}}.
\end{align}
To make our lives a bit easier, we will rescale the moments according to their order like
\begin{equation}
  \label{eq: rescaling the moments}
  \frac{m^*_{\alpha\beta}}{c^{\alpha + \beta}} \rightarrow m^*_{\alpha\beta}, \quad   \frac{m_{\alpha\beta}}{c^{\alpha + \beta}} \rightarrow m_{\alpha\beta}
\end{equation}
to finally get
\begin{equation}
  \sum_{\tau = 0}^\infty \frac{{\Delta t}^\tau }{\tau!} \frac{\partial^\tau}{{\partial t}^\tau} m_{\alpha\beta} =
 \sum_{m,n = 0}^\infty \frac{{(- c\Delta t)}^{m+n}} {m!n!} \frac{\partial^m \partial^n}{ {\partial x}^m{\partial y}^n} m^*_{(\alpha + m)(\beta + n)}.
\end{equation}
This scaling is easily reverted by multiplying with same term again, but most of the time, we will calculate with $c=1$, so the effect of the scaling vanishes completely.
Additionally, this will take out the $c$-term in the aliasing of the moments,~\eqref{eq:aliasing of moments 1} and~\eqref{eq:aliasing of moments 2}, making it a $1:1$ relationship.

For the scale analysis, we introduce a dimensionless scaling parameter $\epsilon$.
Adapting the widely used diffusive scaling, we nondimensionalize the equations with characteristic length and timescales, $L$ and $\iota$
\begin{equation}
  \label{eq: nondimensionalisation}
  \begin{aligned}
    \Delta x & = L\epsilon \\
    \Delta t & = \iota\epsilon^2 \\
    c & = \frac{L}{\iota\epsilon} \\
    \{x, y\} & \rightarrow \{\frac{x}{L}, \frac{y}{L}\} \\
    t & \rightarrow \frac{t}{\iota}.
  \end{aligned}
\end{equation}
Additionally, the moments are expanded according to the scale $\epsilon$
\begin{align}
    \label{eq: expansion of m}
    m_{\alpha\beta} & = \sum_{p=0}^{\infty} \epsilon^p m_{\alpha\beta}^{(p)} \\
    \label{eq: expansion of m star}
    m^*_{\alpha\beta} & = \sum_{p=0}^{\infty} \epsilon^p m_{\alpha\beta}^{*(p)}.
\end{align}
Those are still dependent of space and time, but as they are separated on their length scales, their spatial part is not allowed to depend on $\epsilon$ neither implicitly nor explicitly.
Inserting~\eqref{eq: nondimensionalisation},~\eqref{eq: expansion of m} and~\eqref{eq: expansion of m star} into~\eqref{eq: Taylor of moments} yields

\begin{align}
  \phantom{\equivalent\qquad}
  &\begin{aligned}
  \nonumber
    \mathllap{\equivalent\qquad} & \sum_{\tau = 0}^\infty \frac{{\Delta t}^\tau }{\tau!}  \frac{\partial^\tau}{{\partial t}^\tau} \sum_{p=0}^{\infty} \epsilon^p m_{\alpha\beta}^{(p)} \\
    = &{}\sum_{m,n = 0}^\infty \frac{{(-c\Delta t)}^{m+n}} {m!n!} \frac{\partial^m \partial^n}{ {\partial x}^m{\partial y}^n} \sum_{p=0}^{\infty} \epsilon^p m_{(\alpha + m)(\beta + n)}^{*(p)}
  \end{aligned}\\
  %
  &\begin{aligned}
    \label{eq: nondimensionalised expansion series}
    \mathllap{\equivalent\qquad} &
    \sum_{\tau = 0}^\infty \frac{{(\iota\epsilon^2)}^\tau }{\tau!} \frac{\partial^\tau}{{\partial t}^\tau \iota^\tau} \sum_{p=0}^{\infty} \epsilon^p m_{\alpha\beta}^{(p)} \\
    = &{}\sum_{m,n = 0}^\infty \frac{{(-\frac{L}{\iota\epsilon}(\iota\epsilon^2))}^{m+n}} {m!n!}
    \frac{\partial^m \partial^n}{ {\partial x}^m{\partial y}^n L^{m+n}} \sum_{p=0}^{\infty} \epsilon^p m_{(\alpha + m)(\beta + n)}^{*(p)}
  \end{aligned} \\
 %
  &\begin{aligned}
  \nonumber
    \mathllap{\equivalent\qquad} &
    \sum_{\tau = 0}^\infty \frac{\epsilon^{2\tau} }{\tau!} \frac{\partial^\tau}{{\partial t}^\tau} \sum_{p=0}^{\infty} \epsilon^p m_{\alpha\beta}^{(p)} \\
    = &{}\sum_{m,n = 0}^\infty \frac{{(-\epsilon)}^{m+n}} {m!n!}
    \frac{\partial^m \partial^n}{ {\partial x}^m{\partial y}^n } \sum_{p=0}^{\infty} \epsilon^p m_{(\alpha + m)(\beta + n)}^{*(p)}
  \end{aligned} \\
 %
  &\begin{aligned}
    \label{eq: final nondimensionalised expansion series}
    \mathllap{\equivalent\qquad} &
    \sum_{\tau, p = 0}^\infty\epsilon^{2\tau + p} \frac{1} {\tau!} \frac{\partial^\tau}{{\partial t}^\tau} m_{\alpha\beta}^{(p)} \\
    = &{} \sum_{m,n,p' = 0}^\infty  \epsilon^{m+n+p'} \frac{{(-1)}^{m+n}} {m!n!}
    \frac{\partial^m \partial^n}{ {\partial x}^m{\partial y}^n } m_{(\alpha + m)(\beta + n)}^{*(p')}
  \end{aligned}
\end{align}
Where in~\eqref{eq: final nondimensionalised expansion series}, the summation indices are changed to be unique for better recognition.
