% !TEX root = ../thesis.tex
With the new informations of the last section, we can simplify the cumulant expansions~\eqref{eq: expansions of cumulants zeroth order raw} through~\eqref{eq: expansions of cumulants second order raw} to their final form.

The zeroth order expansions can be worked on using equations~\eqref{eq: eq moments 11_0} through~\eqref{eq: eq moments 22_0} together with equations~\eqref{eq: zeroth order invariant} and~\eqref{eq: first order invariant} to give
\begin{equation}
  \label{eq: expansions of cumulants zeroth order}
  \begin{aligned}
    K_{10}^{(0)} =&\ m_{10}^{(0)} = 0\\
    K_{01}^{(0)} =&\ m_{01}^{(0)} = 0\\
    K_{11}^{(0)} =&\ m_{11}^{(0)} = 0\\
    K_{20}^{(0)} =&\ m_{20}^{(0)} = c_s^2 m_{00}^{(0)}\\
    K_{02}^{(0)} =&\ m_{02}^{(0)} = c_s^2 m_{00}^{(0)}\\
    K_{21}^{(0)} =&\ m_{21}^{(0)} = 0\\
    K_{12}^{(0)} =&\ m_{12}^{(0)} = 0\\
    K_{22}^{(0)} =&\ m_{22}^{(0)} - \frac{ m_{20}^{(0)} m_{02}^{(0)} }{m_{00}^{(0)}} - 2\frac{ m_{11}^{{(0)}^2}}{m_{00}^{(0)}} = 0.
  \end{aligned}
\end{equation}
For the first order terms we will use again~\eqref{eq: eq moments 11_0} through~\eqref{eq: eq moments 02_0} together with~\eqref{eq: eq moments 21_1} and~\eqref{eq: eq moments 12_1} to finally give
\begin{equation}
  \label{eq: expansions of cumulants first order}
  \begin{aligned}
    K_{10}^{(1)} =&\ m_{10}^{(1)}\\
    K_{01}^{(1)} =&\ m_{01}^{(1)}\\
    K_{11}^{(1)} =&\ m_{11}^{(1)} = 0 \\
    K_{20}^{(1)} =&\ m_{20}^{(1)} = 0\\
    K_{02}^{(1)} =&\ m_{02}^{(1)} = 0\\
    K_{21}^{(1)} =&\ m_{21}^{(1)}
    - c_s^2 m_{01}^{(1)} = 0 \\
    K_{12}^{(1)} =&\ m_{21}^{(1)}
    - c_s^2 m_{10}^{(1)} = 0 \\
    K_{22}^{(1)} =&\ m_{22}^{(1)} = 0
  \end{aligned}
\end{equation}
Whats remaining is the expansion of the second order terms.
Here, only the expansion of $K_{22}$ can be simplified, using the same equations like in the derivation of~\eqref{eq: expansions of cumulants first order}.
Be aware, that the second order terms in equation~\eqref{eq: eq moments 11_2} and following cannot be replaced by the nonequilibrium terms.
Hence, we get
\begin{equation}
  \label{eq: expansions of cumulants second order}
  \begin{aligned}
    K_{10}^{(2)} =&\ m_{10}^{(2)} = 0\\
    K_{01}^{(2)} =&\ m_{01}^{(2)} = 0\\
    K_{11}^{(2)} =&\ m_{11}^{(2)} - \frac{ m_{10}^{(1)}m_{01}^{(1)}}{m_{00}^{(0)}} \\
    K_{20}^{(2)} =&\ m_{20}^{(2)} - \frac{ m_{10}^{{(1)}^2}}{m_{00}^{(0)}} \\
    K_{02}^{(2)} =&\ m_{02}^{(2)} - \frac{ m_{01}^{{(1)}^2}}{m_{00}^{(0)}} \\
    K_{12}^{(2)} =&\ m_{12}^{(2)} = 0\\
    K_{21}^{(2)} =&\ m_{21}^{(2)} = 0\\
    K_{22}^{(2)}
    = &\
    m_{22}^{(2)}
    \\&
    - 2 c_s^2 \frac{ m_{10}^{{(1)}^2} }{m_{00}^{(0)}}
    - 2 c_s^2 \frac{ m_{01}^{{(1)}^2} }{m_{00}^{(0)}}
    \\&
    - c_s^2 m_{02}^{(2)}
    - c_s^2 m_{20}^{(2)}
    + c_s^4 m_{00}^{(2)}
    \\&
    + 2 c_s^2\frac{ m_{10}^{{(1)}^2} }{m_{00}^{(0)}}
    + 2 c_s^2\frac{ m_{01}^{{(1)}^2} }{m_{00}^{(0)}}
    \\= &\
    m_{22}^{(2)}
    + c_s^2\left(c_s^2 m_{00}^{(2)}
    - m_{02}^{(2)}
    - m_{20}^{(2)}
    \right)
  \end{aligned}
\end{equation}
