% !TEX root = ../thesis.tex
Following the derivation of $\kappa_{00}$ and $\kappa_{10}$ in~\eqref{eq: definition of kappa_00} and~\eqref{eq: definition of kappa_10}, we calculate the remaining cumulants like
\begin{align*}
  \phantom{\kappa_{11}}
  &\begin{aligned}
  \nonumber
    \mathllap{\kappa_{11}} & = \left.\partial_1 \partial_2 \ln(F) \right|_{\Xi = 0} \\
    & = \left.\partial_2 \left( \frac{1}{F} \partial_1 F \right) \right|_{\Xi = 0} \\
    & = \left.\left( -\frac{1}{F^2} \partial_2 F \partial_1 F + \frac{1}{F} \partial_1\partial_2 F \right) \right|_{\Xi = 0} \\
    & = \left(
      - \frac{1}{m_{00}} m_{01} m_{10}
      + \frac{1}{m_{00}} m_{11}
      \right) \\
    & = \frac{m_{11}}{m_{00}} - \frac{m_{10}m_{01}}{m_{00}^2}
  \end{aligned} \\
  \\
  &\begin{aligned}
  \nonumber
  \mathllap{\kappa_{20}} & = \left.\partial_1^2 \ln(F) \right|_{\Xi = 0} \\
  & =  \left.\partial_1 \left( \frac{1}{F} \partial_1 F \right) \right|_{\Xi = 0} \\
  & =  \left.\left( -\frac{1}{F^2} {(\partial_1 F)}^2 + \frac{1}{F} \partial_1^2 F \right) \right|_{\Xi = 0} \\
  & =  \left(
    - \frac{1}{m_{00}^2} m_{10}^2
    + \frac{1}{m_{00}} m_{20}
    \right)\\
  & = \frac{m_{20}}{m_{00}} - \frac{m_{10}^2}{m_{00}^2}
  \end{aligned} \\
  \\
  &\begin{aligned}
  \nonumber
  \mathllap{\kappa_{21}} & =  \left. \partial_2 \partial_1^2 \ln(F) \right|_{\Xi = 0} \\
  & =  \left.\left(\partial_2\left( -\frac{1}{F^2} {(\partial_1 F)}^2 + \frac{1}{F} \partial_1^2 F \right)\right) \right|_{\Xi = 0} \\
  & =  \left.\left(
      \frac{2}{F^3} \partial_2 F {(\partial_1 F)}^2
    - \frac{2}{F^2} \partial_1 F \partial_1 \partial_2 F
    - \frac{1}{F^2} \partial_2 F \partial_1^2 F
    + \frac{1}{F} \partial_2 \partial_1^2 F
    \right)\right|_{\Xi = 0}\\
  & =  \Bigg(
      \frac{2}{m_{00}^3} m_{01} m_{10}^2
    - \frac{2}{m_{00}^2} m_{10} m_{11}
    \\ &\qquad\qquad
    - \frac{1}{m_{00}^2} m_{01} m_{20}
    + \frac{1}{m_{00}} m_{21}
    \Bigg)\\
  & = \frac{m_{21}}{m_{00}} - \frac{m_{20}m_{01}}{m_{00}^2}
       - 2\frac{m_{10}m_{11}}{m_{00}^2} + 2\frac{m_{10}^2 m_{01}}{m_{00}^3}
  \end{aligned}\\
  \\
  &\begin{aligned}
  \nonumber
  \mathllap{\kappa_{22}} & = \left. \partial_2^2 \partial_1^2 \ln(F) \right|_{\Xi = 0} \\
  & =  \Bigg(\partial_2\Big(
      \frac{2}{F^3} \partial_2 F {(\partial_1 F)}^2
    - \frac{2}{F^2} \partial_1 F \partial_1 \partial_2 F
    - \frac{1}{F^2} \partial_2 F \partial_1^2 F
    + \frac{1}{F} \partial_2 \partial_1^2 F
    \Big)\Bigg)\Bigg|_{\Xi = 0}\\
  %
  & = \bigg(
    - \frac{6}{F^4} {(\partial_2 F)}^2 {(\partial_1 F)}^2
    + \frac{2}{F^3} \partial_2^2 F {(\partial_1 F)}^2
    + \frac{4}{F^3} \partial_1 F \partial_2 F \partial_1 \partial_2 F \\
  & \qquad\qquad\quad
    + \frac{4}{F^3} \partial_1 F \partial_2 F \partial_1 \partial_2 F
    - \frac{2}{F^2} {(\partial_1 \partial_2 F)}^2
    - \frac{2}{F^2} \partial_1 F \partial_1 \partial_2^2 F \\
  & \qquad\qquad\quad
    + \frac{2}{F^3} {(\partial_2 F)}^2  \partial_1^2 F
    - \frac{1}{F^2} \partial_1^2 F \partial_2^2 F
    - \frac{1}{F^2} \partial_2 F \partial_2 \partial_1^2 F \\
  & \qquad\qquad\quad
    - \frac{1}{F^2} \partial_2 F \partial_2 \partial_1^2 F
    + \frac{1}{F}   \partial_1^2 \partial_2^2 F
    \bigg)\bigg|_{\Xi = 0} \\
  %
  & = -\frac{6}{m_{00}^4} m_{10}^2 m_{01}^2 \\
  &\quad
    + \frac{1}{m_{00}^3}
      \left(
        2 m_{10}^2 m_{02} + 4 m_{10}m_{11}m_{01}
        + 4 m_{10}m_{11}m_{01} + 2 m_{20}m_{01}^2
      \right) \\
  &\quad
    - \frac{1}{m_{00}^2}
      \left(
        2 m_{11}^2 + 2 m_{10}m_{12} + m_{20}m_{02} + m_{21}m_{01} + m_{21}m_{01}
      \right) \\
  &\quad
    + \frac{1}{m_{00}} m_{22}\\
  %
  & = \frac{1}{m_{00}} m_{22} \\
    &\quad
    - \frac{1}{m_{00}^2}
    \left(
       2 m_{10}m_{12}  + 2 m_{21}m_{01} + 2 m_{11}^2 + m_{20}m_{02}
    \right) \\
    &\quad
    + \frac{2}{m_{00}^3}
      \left(
        m_{10}^2 m_{02} + 4 m_{10}m_{11}m_{01} + m_{20}m_{01}^2
      \right)\\
    &\quad
       - \frac{6}{m_{00}^4} m_{10}^2 m_{01}^2
  \end{aligned}
\end{align*}
