% !TEX root = ../thesis.tex
As mentioned in Section~\ref{sub: Cumulants from central moments}, we need to calculate the other central moments in order to get to the cumulants. We use again the abbreveations from~\eqref{eq: abbreviations for deriving cumulants from moments} and~\eqref{eq: additional abbreviations}.
\begin{align*}
  \phantom{c_{00}}
  &\begin{aligned}
  \nonumber
    \mathllap{c_{20}} & = {(-c)}^{-2} \partial_1 (EL_1)  \bigr|_{\Xi_1=\Xi_2 = 0} \\
    & = {(-c)}^{-2} \big( EL_1^2 + E \partial_1^2\ln(F)\big)  \bigr|_{\Xi_1=\Xi_2 = 0} \\
    & = {(-c)}^{-2} \big( 0 + \underbrace{E \bigr|_{\Xi_1=\Xi_2 = 0}}_{=m_{00}}
    \underbrace{\partial_1^2\ln(F) \bigr|_{\Xi_1=\Xi_2 = 0}}_{={(-c)}^{2}\kappa_{20}} \big) \\
    & = m_{00}\kappa_{20}
  \end{aligned}\\
  %
  &\begin{aligned}
  \nonumber
    \mathllap{c_{11}} & = {(-c)}^{-2} \partial_2 (EL_1) \bigr|_{\Xi_1=\Xi_2 = 0} \\
    & = {(-c)}^{-2} \big( E L_1 L_2 + E \partial_1\partial_2\ln(F) \big)  \bigr|_{\Xi_1=\Xi_2 = 0} \\
    & = m_{00}\kappa_{11}
  \end{aligned}\\
  %
  &\begin{aligned}
  \nonumber
    \mathllap{c_{21}} & = {(-c)}^{-3} \partial_2 \big(EL_1^2 + E \partial_1^2\ln(F)\big)  \bigr|_{\Xi_1=\Xi_2 = 0} \\
    & = {(-c)}^{-3} \big( E L_1^2 L_2 + 2EL_1\partial_1\partial_2\ln(F) \\
      &\qquad\quad\ \ + EL_2 \partial_1^2\ln(F) + E \partial_1^2\partial_2\ln(F) \big)  \bigr|_{\Xi_1=\Xi_2 = 0} \\
    & = m_{00}\kappa_{21}
  \end{aligned}\\
  &\begin{aligned}
  \nonumber
    \mathllap{c_{12}} & = m_{00}\kappa_{12}
  \end{aligned}\\
  %
  &\begin{aligned}
  \nonumber
    \mathllap{c_{22}} & = {(-c)}^{-4} \partial_2 \big( E L_1^2 L_2 + 2EL_1\partial_1\partial_2\ln(F) \\
      &\qquad\qquad\ \ + EL_2 \partial_1^2\ln(F) + E \partial_1^2\partial_2\ln(F) \big)  \bigr|_{\Xi_1=\Xi_2 = 0} \\
    & = {(-c)}^{-4} \big(
      E L_1^2 L_2^2 + E L_2^2 \partial_2^2\ln(F) + 2 E L_1 L_2 \partial_1\partial_2 \ln(F) \\
    & \qquad\quad\ \ +
      2 E L_1 L_2 \partial_1\partial_2 \ln(F) + 2 E \partial_1\partial_2 \ln(F) \partial_1\partial_2 \ln(F) + 2 E L_1 \partial_1\partial_2^2 \ln(F) \\
    & \qquad\quad\ \ +
      E L_2^2 \partial_1^2 \ln(F) + E \partial_1^2 \ln(F) \partial_2^2 \ln(F) + E L_2 \partial_1\partial_2^2 \ln(F) \\
    & \qquad\quad\ \ +
      E L_2 \partial_1^2 \partial_2 \ln(F) + E\partial_1^2\partial_2^2 \ln(F)
      \big) \bigr|_{\Xi_1=\Xi_2 = 0} \\
    & = {(-c)}^{-4} \big(
    0 + 0 + 0 \\
    & \qquad\quad\ \ +
      0 + 2 E \partial_1\partial_2 \ln(F) \partial_1\partial_2 \ln(F) + 0 \\
    & \qquad\quad\ \ +
      0 + E \partial_1^2 \ln(F) \partial_2^2 \ln(F) + 0 \\
    & \qquad\quad\ \ +
      0 + E\partial_1^2\partial_2^2 \ln(F)
      \big) \bigr|_{\Xi_1=\Xi_2 = 0} \\
    & = m_{00}(\kappa_{22} + 2\kappa_{11}^2 + \kappa_{20}\kappa_{02})
  \end{aligned}
\end{align*}
