% !TEX root = ../thesis.tex

\subsection{\texorpdfstring{$K_{20}$}{K 20} and \texorpdfstring{$K_{02}$}{K 02}}
\label{sub: K 20}
Going further to $K_{20}$, we get with the same reasoning
\begin{equation}
  \begin{aligned}
    K_{20} & = m_{20} - \frac{m_{10}^2}{m_{00}}\\
    \Leftrightarrow
    \sum_{i=0}^\infty \epsilon^i K_{20}^{(i)}
    & = \sum_{i=0}^\infty \epsilon^i m_{20}^{(i)} -
    \frac{\sum_{i,j=0}^\infty \epsilon^{i+j} m_{10}^{(i)}m_{10}^{(j)}}
        {m_{00}^{(0)}}
    \sum_{j=0}^\infty {\left(\sum_{i=1}^\infty \epsilon^i \frac{ - m_{00}^{(i)}}{ m_{00}^{(0)}}\right)}^j
  \end{aligned}
\end{equation}
As before, the zeroth and first order terms of the cumulant and corresponding moment coincide.
For the second order terms, we get
\begin{equation}
  K_{20}^{(2)} = m_{20}^{(2)}
  - \frac{ m_{10}^{{(1)}^2}}{m_{00}^{(0)}},
\end{equation}
and consequently
\begin{equation}
  K_{02}^{(2)} = m_{02}^{(2)}
  - \frac{ m_{01}^{{(1)}^2}}{m_{00}^{(0)}}.
\end{equation}

\subsection{\texorpdfstring{$K_{21}$}{K 21} and \texorpdfstring{$K_{12}$}{K 12}}
\label{sub: K 21}
As before, we take the defining equation for the normalized cumulant, in this case~\eqref{eq: K 21 from moments}, and plug in all expansions with the geometric series expansion like in~\eqref{eq: first expansion}.

\begin{equation}
  \begin{aligned}
    \sum_{i=0}^\infty \epsilon^i K_{21}^{(i)}
    & = \sum_{i=0}^\infty \epsilon^i m_{21}^{(i)}
    \\ &\quad
    - \frac{\sum_{i,j=0}^\infty \epsilon^{i+j} m_{20}^{(i)} m_{01}^{(j)}}{m_{00}^{(0)}}
      \sum_{j=0}^\infty {\left(\sum_{i=1}^\infty \epsilon^i \frac{ - m_{00}^{(i)}}{ m_{00}^{(0)}}\right)}^j
    \\ &\quad
     - 2\frac{\sum_{i,j=0}^\infty \epsilon^{i+j} m_{10}^{(i)} m_{11}^{(j)}}{m_{00}^{(0)}}
      \sum_{j=0}^\infty {\left(\sum_{i=1}^\infty \epsilon^i \frac{ - m_{00}^{(i)}}{ m_{00}^{(0)}}\right)}^j
     \\ &\quad
     + 2\frac{\sum_{i,j,k=0}^\infty \epsilon^{i+j+k} m_{10}^{(i)} m_{10}^{(j)} m_{01}^{(k)}}{m_{00}^{(0)2}}
      {\left(
        \sum_{j=0}^\infty {\left(\sum_{i=1}^\infty \epsilon^i \frac{ - m_{00}^{(i)}}{ m_{00}^{(0)}}\right)}^j
      \right)}^2\\
   \end{aligned}
\end{equation}
Collecting the zeroth order terms, we find again

\begin{equation}
  K_{21}^{(0)} = m_{21}^{(0)}.
\end{equation}
In contrary to the aforementioned, the first order expansions differ:

\begin{equation}
  \begin{aligned}
    K_{21}^{(1)} & = m_{21}^{(1)}
    - \frac{m_{20}^{(0)} m_{01}^{(1)}}{m_{00}^{(0)}}
    \\ &
    = m_{21}^{(1)} - \theta m_{01}^{(1)}
  \end{aligned}
\end{equation}

\subsection{\texorpdfstring{$K_{22}$}{K 22}}
\label{sub: K 22}
The procedure is now well known,~\eqref{eq: K 22 from moments} is expanded into the series.

\begin{equation}
  \begin{aligned}
  \sum_{i=0}^\infty \epsilon^i K_{22}^{(i)}
  & = \sum_{i=0}^\infty \epsilon^i m_{22}^{(i)}
  \\& \quad
  - 2 \frac{ \sum_{i,j=0}^\infty \epsilon^{i+j} m_{10}^{(i)} m_{12}^{(j)} }{m_{00}^{(0)}}
   \sum_{j=0}^\infty {\left(\sum_{i=1}^\infty \epsilon^i \frac{ - m_{00}^{(i)}}{ m_{00}^{(0)}}\right)}^j
  \\& \quad
  - 2 \frac{ \sum_{i,j=0}^\infty \epsilon^{i+j} m_{21}^{(i)} m_{01}^{(j)} }{m_{00}^{(0)}}
   \sum_{j=0}^\infty {\left(\sum_{i=1}^\infty \epsilon^i \frac{ - m_{00}^{(i)}}{ m_{00}^{(0)}}\right)}^j
  \\& \quad
  - 2 \frac{ \sum_{i,j=0}^\infty \epsilon^{i+j} m_{11}^{(i)} m_{11}^{(j)} }{m_{00}^{(0)}}
   \sum_{j=0}^\infty {\left(\sum_{i=1}^\infty \epsilon^i \frac{ - m_{00}^{(i)}}{ m_{00}^{(0)}}\right)}^j
  \\& \quad
  -   \frac{ \sum_{i,j=0}^\infty \epsilon^{i+j} m_{20}^{(i)} m_{02}^{(j)} }{m_{00}^{(0)}}
   \sum_{j=0}^\infty {\left(\sum_{i=1}^\infty \epsilon^i \frac{ - m_{00}^{(i)}}{ m_{00}^{(0)}}\right)}^j
  \\& \quad
  + 2 \frac{ \sum_{i,j,k=0}^\infty \epsilon^{i+j+k} m_{10}^{(i)}m_{10}^{(j)}m_{02}^{(k)} }
  {m_{00}^{(0)2}}
   {\left(
     \sum_{j=0}^\infty {\left(\sum_{i=1}^\infty \epsilon^i \frac{ - m_{00}^{(i)}}{ m_{00}^{(0)}}\right)}^j
   \right)}^2
  \\& \quad
  + 8 \frac{ \sum_{i,j,k=0}^\infty \epsilon^{i+j+k} m_{10}^{(i)}m_{11}^{(j)}m_{01}^{(k)} }
  {m_{00}^{(0)2}}
   {\left(
     \sum_{j=0}^\infty {\left(\sum_{i=1}^\infty \epsilon^i \frac{ - m_{00}^{(i)}}{ m_{00}^{(0)}}\right)}^j
   \right)}^2
  \\& \quad
  + 2 \frac{ \sum_{i,j,k=0}^\infty \epsilon^{i+j+k} m_{20}^{(i)}m_{01}^{(j)}m_{01}^{(k)} }
  {m_{00}^{(0)2}}
   {\left(
     \sum_{j=0}^\infty {\left(\sum_{i=1}^\infty \epsilon^i \frac{ - m_{00}^{(i)}}{ m_{00}^{(0)}}\right)}^j
   \right)}^2
  \\& \quad
  - 6 \frac{ \sum_{i,j,k,l=0}^\infty \epsilon^{i+j+k+l} m_{10}^{(i)}m_{10}^{(j)}m_{01}^{(k)}m_{01}^{(l)}}{m_{00}^{(0)3}}
   {\left(
     \sum_{j=0}^\infty {\left(\sum_{i=1}^\infty \epsilon^i \frac{ - m_{00}^{(i)}}{ m_{00}^{(0)}}\right)}^j
   \right)}^3
   \end{aligned}
 \end{equation}
This time, even the zeroth order moment differs from the cumulant.
\begin{equation}
  K_{22}^{(0)}
  = m_{22}^{(0)} - \frac{ m_{20}^{(0)} m_{02}^{(0)} }{m_{00}^{(0)}} - 2\frac{ m_{11}^{(0)2}  }{m_{00}^{(0)}} = m_{22}^{(0)} - \theta^2 m_{00}^{(0)} - 2\frac{ m_{11}^{(0)2}  }{m_{00}^{(0)}}
 \end{equation}
and the first order terms are
\begin{equation}
  \begin{aligned}
    K_{22}^{(1)}
    & = m_{22}^{(1)}
      - 2\frac{ m_{10}^{(1)} m_{12}^{(0)} }{m_{00}^{(0)}}
      - 2\frac{ m_{21}^{(0)} m_{01}^{(1)} }{m_{00}^{(0)}}
      - 4\frac{ m_{11}^{(1)} m_{11}^{(0)} }{m_{00}^{(0)}}
      - \frac{ m_{20}^{(0)} m_{02}^{(1)} }{m_{00}^{(0)}}
      - \frac{ m_{20}^{(1)} m_{02}^{(0)} }{m_{00}^{(0)}}
    \\& = m_{22}^{(1)}
      - \theta (m_{20}^{(1)} + m_{02}^{(1)})
      - 2\frac{ m_{10}^{(1)} m_{12}^{(0)} }{m_{00}^{(0)}}
      - 2\frac{ m_{21}^{(0)} m_{01}^{(1)} }{m_{00}^{(0)}}
      - 4\frac{ m_{11}^{(1)} m_{11}^{(0)} }{m_{00}^{(0)}}
  \end{aligned}
 \end{equation}
