\documentclass{article}
\usepackage[utf8]{inputenc}
\usepackage{definitions}

\begin{document}
  \paragraph{Expansions}
  \begin{align}
      K_{21}^{(0)} & = 0 \label{E1}\tag{E1}\\
      K_{22}^{(0)} & = -\theta m_{00}^{(0)}\label{E2}\tag{E2}\\
      K_{11}^{(1)} & = m_{11}^{(1)} \label{E3}\tag{E3}\\
      K_{20}^{(1)} & = m_{20}^{(1)} \label{E4}\tag{E4}\\
      K_{02}^{(1)} & = m_{02}^{(1)} \label{E5}\tag{E5}\\
      K_{21}^{(1)} & = m_{21}^{(1)} - \theta m_{01}^{(1)} \label{E6}\tag{E6}\\
      K_{12}^{(1)} & = m_{12}^{(1)} - \theta m_{10}^{(1)} \label{E7}\tag{E7}\\
      K_{22}^{(1)} & = m_{22}^{(1)} - \theta (m_{20}^{(1)} + m_{02}^{(1)}) \label{E8}\tag{E8}\\
      K_{11}^{(2)} & = m_{11}^{(2)} - \frac{ m_{10}^{(1)}m_{01}^{(1)}}{m_{00}^{(0)}}. \label{E9}\tag{E9}\\
      K_{20}^{(2)} & = m_{20}^{(2)} - \frac{ m_{10}^{(1)2}}{m_{00}^{(0)}} \label{E10}\tag{E10}\\
      K_{02}^{(2)} & = m_{02}^{(2)} - \frac{ m_{01}^{(1)2}}{m_{00}^{(0)}} \label{E11}\tag{E11}
  \end{align}

  \paragraph{prerquesites}
  \begin{align}
    m_{00} &= m_{00}^*  \label{P1}\tag{P1}\\
    m_{00}^{(p)} &= m_{00}^{*(p)} \label{P2}\tag{P2} \\
    m_{\alpha\beta}^{(1)} &= m_{\alpha\beta}^{*(1)} \label{P3}\tag{P3} \\
    m_{\alpha\beta}^{(0)} &= m_{\alpha\beta}^{*(0)} \label{P4}\tag{P4} \\
    \partial_x m_{\alpha\beta}^{(0)} &= 0  \label{P5}\tag{P5}\\
    \partial_y m_{\alpha\beta}^{(0)} &= 0  \label{P6}\tag{P6}
  \end{align}

  \paragraph{reduced case}
  \begin{align}
    m_{11}^{(1)*} & = (1-\omega_1) m_{11}^{(1)}\label{R1}\tag{R1} \\
    m_{20}^{(1)*} - m_{02}^{(1)*}
      & = (1-\omega_1) (m_{20}^{(1)} - m_{02}^{(1)})\label{R2}\tag{R2} \\
    m_{20}^{(1)*} + m_{02}^{(1)*}
      & =  \frac{2 m_{00}^{(1)}}{3}\label{R3}\tag{R3} \\
    m_{21}^{(1)*} & = \theta m_{01}^{(1)*}\label{R4}\tag{R4} \\
    m_{12}^{(1)*} & = \theta m_{10}^{(1)*}\label{R5}\tag{R5} \\
    m_{22}^{(1)*} & = \theta (m_{20}^{(1)*} + m_{02}^{(1)*}) = \theta \frac{2 m_{00}^{(1)}}{3}\label{R6}\tag{R6} \\
    m_{11}^{(2)*} - \frac{ m_{10}^{(1)*}m_{01}^{(1)*}}{m_{00}^{(0)*}}
    & = (1-\omega_1)\left(m_{11}^{(2)} - \frac{ m_{10}^{(1)}m_{01}^{(1)}}{m_{00}^{(0)}}\right)\label{R7}\tag{R7} \\
    m_{20}^{(2)*}-m_{02}^{(2)*} - \frac{ m_{10}^{(1)*2} - m_{01}^{(1)*2}}{m_{00}^{(0)*}}
    & = (1-\omega_1) \left(m_{20}^{(2)}-m_{02}^{(2)} - \frac{ m_{10}^{(1)2} - m_{01}^{(1)2}}{m_{00}^{(0)}}\right)\label{R8}\tag{R8} \\
    %
    m_{20}^{(2)*}+m_{02}^{(2)*} - \frac{ m_{10}^{(1)*2} + m_{01}^{(1)*2}}{m_{00}^{(0)*}}
    & = \frac{2 m_{00}^{(2)}}{3} \label{R9}\tag{R9} \\
    \text{\eqref{R8}+\eqref{R9}:}\quad2m_{20}^{(2)*}
    & = (1-\omega_1) (m_{20}^{(2)}-m_{02}^{(2)})\nonumber \\
    &\quad+ (1+\omega_1)\frac{ m_{10}^{(1)2} - m_{01}^{(1)2}}{m_{00}^{(0)}} + \frac{2 m_{00}^{(2)}}{3}\label{R10}\tag{R10} \\
    m_{11}^{(2)*}
    & = (1-\omega_1)m_{11}^{(2)} + \omega_1 \frac{ m_{10}^{(1)}m_{01}^{(1)}}{m_{00}^{(0)}}\label{R11}\tag{R11} \\
    m_{11}^{(2)}
    & = \frac{1}{(1-\omega_1)}m_{11}^{(2)*} + \frac{\omega_1}{(1-\omega_1)} \frac{ m_{10}^{(1)}m_{01}^{(1)}}{m_{00}^{(0)}}\label{R12}\tag{R12}
  \end{align}

  \paragraph{equilibrium}
  \begin{align}
    m_{00}^{eq(0)} & = 0 \label{Q1}\tag{Q1} \\
    m_{11}^{eq(1)} & = 0 \label{Q2}\tag{Q2} \\
    m_{20}^{eq(1)} & = \frac{1}{3} m_{00}^{(1)} \label{Q3}\tag{Q3} \\
    m_{02}^{eq(1)} & = \frac{1}{3} m_{00}^{(1)}  \label{Q4}\tag{Q4} \\
    m_{21}^{eq(1)} & = \theta m_{01}^{eq(1)} \label{Q5}\tag{Q5} \\
    m_{12}^{eq(1)} & = \theta m_{10}^{eq(1)} \label{Q6}\tag{Q6} \\
    m_{22}^{eq(1)} & = \theta (m_{20}^{eq(1)} + m_{02}^{eq(1)}) \label{Q7}\tag{Q7} \\
    m_{11}^{eq(2)} & = \frac{ m_{10}^{eq(1)}m_{01}^{eq(1)}}{m_{00}^{eq(0)}} \label{Q8}\tag{Q8} \\
    m_{20}^{eq(2)} - \frac{ m_{10}^{eq(1)2}}{m_{00}^{eq(0)}} & = \frac{1}{3} m_{00}^{(2)} \label{Q9}\tag{Q9} \\
    m_{02}^{eq(2)} - \frac{ m_{01}^{eq(1)2}}{m_{00}^{eq(0)}} & = \frac{1}{3} m_{00}^{(2)} \label{Q10}\tag{Q10}
  \end{align}

  \paragraph{mass conservation}
  \begin{align}
    \partial_t m_{00}^{(0)}  & =  - \partial_x m_{10}^{(1)} - \partial_y m_{01}^{(1)}\label{M1}\tag{M1} \\
    \partial_{xx} m_{10}^{(1)}  & = - \partial_{xy} m_{01}^{(1)} \label{M2}\tag{M2}\\
    \partial_{yx} m_{10}^{(1)}  & = - \partial_{yy} m_{01}^{(1)} \label{M3}\tag{M3}
  \end{align}

  \paragraph{base equation}
  \begin{equation}
    \label{B1}\tag{B1}
    \begin{aligned}
       \partial_t m_{10}^{(1)} & =
      m_{10}^{*(3)} - m_{10}^{(3)} - \partial_x m_{20}^{*(2)} \\
      &\quad - \partial_y m_{11}^{*(2)} + \frac{1}{2}\partial_{xx} m_{30}^{*(1)} + \frac{1}{2} \partial_{yy} m_{12}^{*(1)} + \partial_{xy} m_{21}^{*(1)}
    \end{aligned}
  \end{equation}

  \paragraph{auxiliary equations}
  \begin{align}
    m_{20}^{(2)} + \partial_t m_{20}^{(0)} + \partial_y m_{21}^{*(1)} + \partial_x m_{30}^{*(1)} &= m_{20}^{*(2)} \label{A1}\tag{A1} \\
    m_{11}^{(2)} + \partial_t m_{11}^{(0)} + \partial_y m_{12}^{*(1)} + \partial_x m_{21}^{*(1)} &= m_{11}^{*(2)} \label{A2}\tag{A2}
  \end{align}

  \paragraph{combined}~\eqref{A1}$+$\eqref{R10}
  \begin{equation*}
    \begin{aligned}
      2m_{20}^{(2)} + 2\partial_t m_{20}^{(0)} + 2\partial_y m_{21}^{*(1)} + 2\partial_x m_{30}^{*(1)}
      &= (1-\omega_1) (m_{20}^{(2)}-m_{02}^{(2)})
      \\&\quad
      + (1+\omega_1)\frac{ m_{10}^{(1)2} - m_{01}^{(1)2}}{m_{00}^{(0)}} + \frac{2 m_{00}^{(2)}}{3}
    \end{aligned}
  \end{equation*}
  with~\eqref{R4} and~\eqref{P3}
  \begin{equation}
    \label{C1}\tag{C1}
    \begin{aligned}
      m_{20}^{(2)} &= \frac{1}{2}(1-\omega_1) (m_{20}^{(2)}-m_{02}^{(2)})
      + \frac{1}{2}(1+\omega_1)\frac{ m_{10}^{(1)2} - m_{01}^{(1)2}}{m_{00}^{(0)}} + \frac{ m_{00}^{(2)}}{3}
      \\&\quad
      - \partial_t m_{20}^{(0)} - \theta\partial_y m_{01}^{(1)} - \partial_x m_{10}^{(1)}
    \end{aligned}
  \end{equation}
  \paragraph{combined}~\eqref{A2}$+$\eqref{R11}
  \begin{equation*}
    m_{11}^{(2)} + \partial_t m_{11}^{(0)} + \partial_y m_{12}^{*(1)} + \partial_x m_{21}^{*(1)} = (1-\omega_1)m_{11}^{(2)} + \omega_1 \frac{ m_{10}^{(1)}m_{01}^{(1)}}{m_{00}^{(0)}}
  \end{equation*}
  with~\eqref{R4},~\eqref{R5} and~\eqref{P3}
  \begin{equation}
    \label{C2}\tag{C2}
    m_{11}^{(2)} = (1-\omega_1)m_{11}^{(2)} + \omega_1 \frac{ m_{10}^{(1)}m_{01}^{(1)}}{m_{00}^{(0)}}  - \partial_t m_{11}^{(0)} - \theta\partial_y m_{10}^{(1)} - \theta\partial_x m_{01}^{(1)}
  \end{equation}
\end{document}
